src/type/Env.v
@@ -20,7 +20,47 @@ End FnType.
 Module EnvType.
   Definition t := IdMap.t FnType.t.
 
-  Inductive judge (envt: EnvType.t) (labs: Ensemble Label) (s: list Stmt) : Prop :=
+  Inductive ro_judge (envt: t) (s: list Stmt) : Prop :=
+  | ro_empty
+    (STMT: s = [])
+  | ro_assign
+    r e
+    (STMT: s = [stmt_assign r e])
+  | ro_load
+    r e
+    (STMT: s = [stmt_pload r e])
+  | ro_alloc
+    r e
+    (STMT: s = [stmt_palloc r e])
+  | ro_loop
+    r e s
+    (BODY: ro_judge envt s)
+    (STMT: s = [stmt_loop r e s])
+  | ro_continue
+    e
+    (STMT: s = [stmt_continue e])
+  | ro_break
+    (STMT: s = [stmt_break])
+  | ro_call
+    r f e
+    (F_TYPE: IdMap.find f envt = Some FnType.RO)
+    (STMT: s = [stmt_call r f e])
+  | ro_return
+    e
+    (STMT: s = [stmt_return e])
+  | ro_seq
+    s_l s_r
+    (LEFT: ro_judge envt s_l)
+    (RIGHT: ro_judge envt s_r)
+    (STMT: s = s_l ++ s_r)
+  | ro_if_then_else
+    s_t s_f e
+    (TRUE: ro_judge envt s_t)
+    (FALSE: ro_judge envt s_f)
+    (STMT: s = [stmt_if e s_t s_f])
+  .
+
+  Inductive rw_judge (envt: t) (labs: Ensemble Label) (s: list Stmt) : Prop :=
   | rw_empty
     (LABS: labs = Empty_set _)
     (STMT: s = [])
@@ -44,17 +84,23 @@ Module EnvType.
     (LABS: labs = Singleton _ lab)
     (STMT: s = [stmt_pcas r e_loc e_old e_new (mid ++ [lab])])
     (* TODO: mid is a variable *)
+  | rw_checkpoint
+    r s_c mid lab
+    (CLOS: ro_judge envt s)
+    (LABS: labs = Singleton _ lab)
+    (STMT: s = [stmt_chkpt r s_c (mid ++ [lab])])
+    (* TODO: mid is a variable *)
   | rw_if_then_else
     labs_t labs_f e s_t s_f
+    (TRUE: rw_judge envt labs_t s_t)
+    (FALSE: rw_judge envt labs_f s_f)
     (LABS: labs = Union _ labs_t labs_f)
-    (TRUE: judge envt labs_t s_t)
-    (FALSE: judge envt labs_f s_f)
     (STMT: s = [stmt_if e s_t s_f])
   | rw_seq
     s_l s_r labs_l labs_r
     (DISJ: Disjoint _ labs_l labs_r)
-    (LEFT: judge envt labs_l s_l)
-    (RIGHT: judge envt labs_r s_r)
+    (LEFT: rw_judge envt labs_l s_l)
+    (RIGHT: rw_judge envt labs_r s_r)
     (LABS: labs = Union _ labs_l labs_r)
     (STMT: s = s_l ++ s_r)
   (* TODO: Define other rules *)
@@ -66,14 +112,20 @@ Module TypeSystem.
   | env_empty
     (ENV: env = IdMap.empty _)
     (ENVT: envt = IdMap.empty _)
+  | env_ro
+    env0 envt0
+    s prms f
+    (JUDG: judge env0 envt0)
+    (ROJ: EnvType.ro_judge envt s)
+    (ENV: env = IdMap.add f (prms, s) env0)
+    (ENVT: envt0 = IdMap.add f FnType.RO envt0)
   | env_rw
     env0 envt0
     labs s prms_all prms mid f
     (JUDG: judge env0 envt0)
-    (RWJ: EnvType.judge envt labs s)
+    (RWJ: EnvType.rw_judge envt labs s)
     (PRMS: prms_all = prms ++ [mid])
     (ENV: env = IdMap.add f (prms_all, s) env0)
     (ENVT: envt0 = IdMap.add f FnType.RW envt0)
-  (* TODO: Define ENV-RO *)
   .
 End TypeSystem.
