src/proof/ControlConstructCases.v
@@ -1,0 +1,28 @@
+Require Import Lia.
+Require Import List.
+Import ListNotations.
+
+Require Import sflib.
+
+From Memento Require Import Utils.
+From Memento Require Import Syntax.
+From Memento Require Import Semantics.
+
+Set Implicit Arguments.
+
+Lemma checkpoint_cases :
+  forall env tr s s_term c c_term ts ts_term mmts mmts_term,
+    (exists rmap r mid, c = [Cont.chkptcont rmap r [] mid]) ->
+    Thread.rtc env tr (Thread.mk s c ts mmts) (Thread.mk s_term c_term ts_term mmts_term) [] ->
+  <<CALL_ONGOING:
+    exists c_pfx, c_term = c_pfx ++ c
+    /\ Thread.rtc env tr (Thread.mk s [] ts mmts) (Thread.mk s_term c_pfx ts_term mmts_term) []>>
+  \/
+  <<CALL_DONE:
+    exists s_r c_r ts_r mmts_r e,
+      Thread.rtc env tr (Thread.mk s [] ts mmts) (Thread.mk ((stmt_return e) :: s_r) c_r ts_r mmts_r) []
+      /\ Thread.step env [] (Thread.mk ((stmt_return e) :: s_r) (c_r ++ c) ts_r mmts_r) (Thread.mk s_term c_term ts_term mmts_term)
+      /\ s_term = [] /\ c_term = []>>.
+Proof.
+  admit.
+Qed.
